verification/PacketPile2.dfy
@@ -1,0 +1,100 @@
+// Parallel to PacketPile in PacketPile.dfy
+// Since having objects from another class is a framing nightmare,
+// this file focuses on the 'status' of a BloodPacket 
+
+class PacketPile 
+{
+    var buf: array<int>;  // represents status 
+    var count: int; 
+    var low: int;
+
+    predicate Valid() 
+    reads this, this.buf; 
+    {
+        buf != null && 
+        0 <= count <= buf.Length &&
+        0 <= low <= buf.Length &&
+        forall j :: 0 <= j < count ==> 0 <= buf[j] <= 2 
+        // Valid statuses
+        // 0: clear
+        // 1: almost expired
+        // 2: expired
+    }
+
+    method Init(size: int, low1: int)
+    modifies this; 
+    requires 0 <= low1 <= size; 
+    ensures Valid();
+    ensures fresh(buf);
+    ensures buf.Length == size; 
+    ensures count == 0; 
+    ensures low == low1; 
+    {
+        buf := new int[size];
+        count := 0; // initially 0 packets
+        low := low1; 
+    }
+
+    method getNAlmostExpired() returns (total: int)
+    requires Valid(); ensures Valid()
+    ensures total == Count(buf[..count], 1)
+    {
+        total := 0;
+        var i: int := 0;
+        while (i < count) 
+        invariant 0 <= i <= count;
+        invariant total == Count(buf[..i], 1);
+        {
+            if (buf[i] == 1) 
+            {
+                total := total + 1; 
+            }
+            DistributiveLemma(buf[..i], [buf[i]], 1);
+            assert buf[..i+1] == buf[..i] + [buf[i]];
+            i := i + 1; 
+        }
+    }
+
+    method getAlmostExpired() returns (trash: seq<int>)
+        requires Valid(); ensures Valid()
+        ensures forall i :: 0 <= i < |trash| ==> trash[i] == 1;
+    {
+        var size := getNAlmostExpired();
+        //trash := new int[size];
+        trash := [];
+        var i := 0;
+        var next := 0;
+        while i < count
+        decreases count - i
+        invariant 0 <= i <= count
+        //invariant 1 in buf[..i] <==> next > 0
+        invariant 0 <= next <= i
+        invariant forall j :: 0 <= j < |trash| ==> trash[j] == 1
+        {
+            if buf[i] == 1 {
+                //trash[next] := buf[i];
+                //next := next + 1;
+                trash := trash + [buf[i]];
+            }
+            i := i + 1;
+        }
+    }
+}
+
+function method Count(a: seq<int>, key: int) : nat
+decreases |a|
+{   
+    if |a| == 0 then 0 else
+    (if a[0] == key then 1 else 0) + Count(a[1..], key)
+}
+
+lemma DistributiveLemma(a: seq<int>, b: seq<int>, key: int)
+ensures Count(a + b, key) == Count(a, key) + Count(b, key)
+{
+    if a == [] {
+        assert a + b == b;
+    } else {
+        DistributiveLemma(a[1..], b, key);
+        assert a + b == [a[0]] + (a[1..] + b);
+    }
+}
